Typechecking.v
@@ -1,301 +1,277 @@
-Require Import SGA.Common SGA.Syntax SGA.Environments SGA.Types.
+Require Export SGA.Common SGA.Syntax SGA.Types.
 
 Tactic Notation "teauto" := eauto with types.
 Tactic Notation "teauto" integer(n) := eauto n with types.
 
 Section TC.
-  Notation tenv A := (fenv A type).
+  Context {var_t reg_t fn_t: Type}.
 
-  Context {TVar TFn: Type}.
-  Context (V: fenv nat nat).
-  Context (Sigma: fenv TFn ExternalSignature).
+  Context (GammaEnv: Env var_t type).
+  Context (R: reg_t -> type).
+  Context (Sigma: fn_t -> ExternalSignature).
 
-  Notation rule := (rule TVar TFn).
-  Notation fenv_le := (fenv_le type_le).
+  Notation varenv_t := GammaEnv.(env_t).
+  Notation rule := (rule var_t R Sigma).
+  Notation expr := (expr var_t R Sigma).
 
-  Inductive HasType : forall (Gamma: tenv TVar) (s: rule) (tau: type), Prop :=
-  | HasTypePromote:
-      forall (Gamma: tenv TVar) (s: rule)
-        (tau: type) (tau': type),
-        type_le tau tau' ->
-        HasType Gamma s tau' ->
-        HasType Gamma s tau
-  | HasTypeBind:
-      forall (Gamma: tenv TVar)
-        (var: TVar) (expr: rule) (body: rule)
-        (tau tau': type),
-        HasType Gamma expr tau' ->
-        HasType (fenv_add Gamma var tau') body tau ->
-        HasType Gamma (Bind var expr body) tau
-  | HasTypeVar:
-      forall (Gamma: tenv TVar)
-        (var: TVar)
-        (tau: type),
-        Gamma var tau ->
-        HasType Gamma (Var var) tau
-  | HasTypeSkip:
-      forall (Gamma: tenv TVar),
-        HasType Gamma Skip unit_t
-  | HasTypeConst:
-      forall (Gamma: tenv TVar)
-        (cst: bits),
-        HasType Gamma (Const cst) (bit_t (length cst))
-  | HasTypeIf:
-      forall (Gamma: tenv TVar)
-        (cond: rule) (tbranch: rule) (fbranch: rule)
-        (tau: type),
-        HasType Gamma cond (bit_t 1) ->
-        HasType Gamma tbranch tau ->
-        HasType Gamma fbranch tau ->
-        HasType Gamma (If cond tbranch fbranch) tau
-  | HasTypeFail:
-      forall (Gamma: tenv TVar)
-        (tau: type),
-        HasType Gamma Fail tau
-  | HasTypeRead:
-      forall (Gamma: tenv TVar)
-        (level: Level) (idx: nat)
-        (size: nat) (n: nat),
-        V idx size ->
-        HasType Gamma (Read level idx) (bit_t size)
-  | HasTypeWrite:
-      forall (Gamma: tenv TVar)
-        (level: Level) (idx: nat) (value: rule)
-        (size: nat) (n: nat),
-        V idx size ->
-        HasType Gamma value (bit_t size) ->
-        HasType Gamma (Write level idx value) unit_t
-  | HasTypeCall:
-      forall (Gamma: tenv TVar)
-        (idx: TFn) (args: list rule)
-        (argSizes: list nat) (retSize: nat),
-        Sigma idx (FunSig argSizes retSize) ->
-        List.length args = List.length argSizes ->
-        forall2 (fun arg argSize => HasType Gamma arg (bit_t argSize)) args argSizes ->
-        HasType Gamma (Call idx args) (bit_t retSize).
+  Inductive WellTypedExpr : forall (Gamma: varenv_t) {tau: type} (e: expr tau), Prop :=
+  | WellTypedVar:
+      forall (Gamma: varenv_t)
+        (tau: type) (var: var_t),
+        getenv Gamma var = Some tau ->
+        WellTypedExpr Gamma (Var tau var)
+  | WellTypedConst:
+      forall (Gamma: varenv_t) {n} (cst: bits n),
+        WellTypedExpr Gamma (Const cst)
+  | WellTypedRead:
+      forall (Gamma: varenv_t)
+        (port: Port) (idx: reg_t),
+        WellTypedExpr Gamma (Read port idx)
+  | WellTypedCall:
+      forall (Gamma: varenv_t)
+        (idx: fn_t)
+        (arg1: expr (Sigma idx).(arg1Type))
+        (arg2: expr (Sigma idx).(arg2Type)),
+        WellTypedExpr Gamma arg1 ->
+        WellTypedExpr Gamma arg2 ->
+        WellTypedExpr Gamma (Call idx arg1 arg2).
 
-  Hint Constructors HasType : types.
+  Inductive WellTypedRule : forall (Gamma: varenv_t) {tau: type} (r: rule), Prop :=
+  | WellTypedSkip:
+      forall (Gamma: varenv_t),
+        WellTypedRule Gamma Skip
+  | WellTypedFail:
+      forall (Gamma: varenv_t),
+        WellTypedRule Gamma Fail
+  | WellTypedBind:
+      forall (Gamma: varenv_t)
+        (tau: type) (k: var_t) (ex: expr tau) (body: rule),
+        WellTypedExpr Gamma ex ->
+        WellTypedRule (putenv Gamma k tau) body ->
+        WellTypedRule Gamma (Bind k ex body)
+  | WellTypedIf:
+      forall (Gamma: varenv_t)
+        (cond: expr (bits_t 1)) (tbranch: rule) (fbranch: rule),
+        WellTypedExpr Gamma cond ->
+        WellTypedRule Gamma tbranch ->
+        WellTypedRule Gamma fbranch ->
+        WellTypedRule Gamma (If cond tbranch fbranch)
+  | WellTypedWrite:
+      forall (Gamma: varenv_t)
+        (tau: type) (port: Port) (idx: reg_t) (value: expr tau),
+        WellTypedExpr Gamma value ->
+        WellTypedRule Gamma (Write port idx value).
+
+  Hint Constructors WellTyped : types.
   Hint Extern 1 => unfold forall2 in * : types.
-
-  Lemma HasType_morphism:
-    forall (Gamma1: tenv TVar) s tau,
-      HasType Gamma1 s tau ->
-      forall (Gamma2: tenv TVar),
-        fenv_le Gamma1 Gamma2 ->
-        HasType Gamma2 s tau.
-  Proof.
-    induction 1; intros Gamma2 le; teauto 6.
-    specialize (le _ _ H).
-    firstorder teauto.
-  Qed.
-
-  Hint Resolve HasType_morphism : types.
-  (* Note: no MaxType_morphism, since changing the environment changes the MaxType of the refs *)
-
-  Inductive MaxType : forall (Gamma: tenv TVar) (s: rule) (tau: type), Prop :=
-  | MaxTypeBind:
-      forall (Gamma: tenv TVar)
-        (var: TVar) (expr: rule) (body: rule)
-        (tau tau': type),
-        MaxType Gamma expr tau' ->
-        MaxType (fenv_add Gamma var tau') body tau ->
-        MaxType Gamma (Bind var expr body) tau
-  | MaxTypeVar:
-      forall (Gamma: tenv TVar)
-        (var: TVar)
-        (tau: type),
-        Gamma var tau ->
-        MaxType Gamma (Var var) tau
-  | MaxTypeSkip:
-      forall (Gamma: tenv TVar),
-        MaxType Gamma Skip unit_t
-  | MaxTypeConst:
-      forall (Gamma: tenv TVar)
-        (cst: bits),
-        MaxType Gamma (Const cst) (bit_t (length cst))
-  | MaxTypeIfF:
-      forall (Gamma: tenv TVar)
-        (cond: rule) (tbranch: rule) (fbranch: rule)
-        (tauf taut: type),
-        HasType Gamma cond (bit_t 1) ->
-        MaxType Gamma tbranch taut ->
-        MaxType Gamma fbranch tauf ->
-        type_le tauf taut ->
-        MaxType Gamma (If cond tbranch fbranch) tauf
-  | MaxTypeIfT:
-      forall (Gamma: tenv TVar)
-        (cond: rule) (tbranch: rule) (fbranch: rule)
-        (tauf taut: type),
-        HasType Gamma cond (bit_t 1) ->
-        MaxType Gamma tbranch taut ->
-        MaxType Gamma fbranch tauf ->
-        type_le taut tauf ->
-        MaxType Gamma (If cond tbranch fbranch) taut
-  | MaxTypeFail:
-      forall (Gamma: tenv TVar),
-        MaxType Gamma Fail any_t
-  | MaxTypeRead:
-      forall (Gamma: tenv TVar)
-        (level: Level) (idx: nat)
-        (size: nat) (n: nat),
-        V idx size ->
-        MaxType Gamma (Read level idx) (bit_t size)
-  | MaxTypeWrite:
-      forall (Gamma: tenv TVar)
-        (level: Level) (idx: nat) (value: rule)
-        (size: nat) (n: nat),
-        V idx size ->
-        HasType Gamma value (bit_t size) ->
-        MaxType Gamma (Write level idx value) unit_t
-  | MaxTypeCall:
-      forall (Gamma: tenv TVar)
-        (idx: TFn) (args: list rule)
-        (argSizes: list nat) (retSize: nat),
-        Sigma idx (FunSig argSizes retSize) ->
-        List.length args = List.length argSizes ->
-        forall2 (fun arg argSize => HasType Gamma arg (bit_t argSize)) args argSizes ->
-        MaxType Gamma (Call idx args) (bit_t retSize).
-  (* FIXME use single HasType premise in last three rules? *)
-
-  Hint Constructors MaxType : types.
-
-  Theorem maxtypes_unicity :
-    forall Gamma s tau,
-      MaxType Gamma s tau ->
-      forall tau',
-        MaxType Gamma s tau' ->
-        tau = tau'.
-  Proof.
-    induction 1; intros * HasType';
-      inversion HasType'; subst.
-    1-12: solve [firstorder (subst; firstorder teauto)].
-  Qed.
-
-  Hint Resolve maxtypes_unicity : types.
-
-  Lemma MaxType_HasType : forall Gamma s tau', MaxType Gamma s tau' -> forall tau, type_le tau tau' -> HasType Gamma s tau.
-    induction 1; teauto.
-  Qed.
-
-  Notation "Gamma [ k ↦ v ]" :=
-    (fenv_add Gamma k v) (at level 7, left associativity, format "Gamma [ k  ↦  v ]").
-  Notation "Gamma ⊢ s :: tau" :=
-    (HasType Gamma s tau) (at level 8, no associativity).
-  Notation "Gamma ⊩ s :: tau" :=
-    (MaxType Gamma s tau) (at level 8, no associativity).
-
-  Notation "tau ⩽ tau'" :=
-    (type_le tau tau') (at level 10, no associativity).
-
-  Ltac t :=
-    repeat match goal with
-           | [ H: fn ?Gamma ?k ?v, Hle: fenv_le ?Gamma _ |- _ ] =>
-             pose_once Hle k v H
-           | [ H: exists _, _ |- _ ] => destruct H
-           | [ H: _ /\ _ |- _ ] => destruct H
-           end.
-
-  Lemma MaxType_increasing'' : forall s Gamma tau,
-      MaxType Gamma s tau ->
-      forall (Gamma': tenv TVar),
-        fenv_le Gamma Gamma' ->
-        exists tau',
-          MaxType Gamma' s tau' /\
-          type_le tau tau'.
-  Proof.
-    induction 1; intros * le; t; teauto 6.
-
-    - specialize (IHMaxType1 _ le).
-      t.
-      assert (fenv_le Gamma[var ↦ tau'] Gamma'[var ↦ x]) as Hdiff.
-      { apply fenv_add_increasing; eassumption. }
-      specialize (IHMaxType2 _ Hdiff).
-      t.
-      teauto.
-
-    - specialize (IHMaxType1 _ le).
-      t.
-      specialize (IHMaxType2 _ le).
-      t.
-
-      destruct (type_le_upper_bounds_comparable
-                  tauf taut _ _
-                  ltac:(eassumption)
-                  ltac:(eassumption)
-                  ltac:(eassumption)).
-      teauto.
-      teauto 6.
-
-    - specialize (IHMaxType1 _ le).
-      t.
-      specialize (IHMaxType2 _ le).
-      t.
-
-      destruct (type_le_upper_bounds_comparable
-                  taut tauf _ _
-                  ltac:(eassumption)
-                  ltac:(eassumption)
-                  ltac:(eassumption)).
-      teauto.
-      teauto 6.
-    - teauto 8.
-  Qed.
-
-  Lemma HasType_MaxType : forall Gamma s tau,
-      HasType Gamma s tau ->
-      exists tau', MaxType Gamma s tau' /\ tau ⩽ tau'.
-  Proof.
-    induction 1; try solve [teauto || firstorder teauto].
-    - t.
-
-      pose proof (MaxType_increasing''
-                    _ _ _ H1 Gamma[var ↦ x0]
-                    ltac:(teauto)).
-      t.
-      teauto.
-    - t.
-
-      destruct (type_le_upper_bounds_comparable
-                  tau tau x x0
-                  ltac:(teauto)
-                  ltac:(eassumption)
-                  ltac:(eassumption)).
-      teauto.
-      teauto.
-  Qed.
-
-  Hint Resolve MaxType_HasType : types.
-
-  Theorem types_unicity :
-    forall Gamma s tau,
-      HasType Gamma s tau ->
-      HasType Gamma s any_t \/
-      forall tau', HasType Gamma s tau' -> tau = tau'.
-  Proof.
-    intros Gamma s tau H.
-    pose proof (HasType_MaxType _ _ _ H).
-    t.
-    destruct (type_eq_dec x any_t); subst.
-    - teauto.
-    - right.
-      intros tau' H'.
-      pose proof (HasType_MaxType _ _ _ H').
-      t.
-      assert (x = x0) by teauto; subst.
-
-      transitivity x0.
-      teauto.
-      teauto.
-  Qed.
-
-  Notation scheduler := (scheduler TVar TFn).
-
-  Inductive SchedulerHasTypes: forall (s: scheduler), Prop :=
-  | SchedulerHasTypesDone : SchedulerHasTypes Done
-  | SchedulerHasTypesTry :
-      forall r tau s1 s2,
-        HasType fenv_nil r tau ->
-        SchedulerHasTypes s1 ->
-        SchedulerHasTypes s2 ->
-        SchedulerHasTypes (Try r s1 s2).
 End TC.
+
+(* FIXME: The new uniqueness theorem should say that removing types should be
+          (mostly) injective *)
+
+(*   Inductive MaxType : forall (Gamma: varenv_t) (s: rule) (tau: type), Prop := *)
+(*   | MaxTypeBind: *)
+(*       forall (Gamma: varenv_t) *)
+(*         (var: var_t) (expr: rule) (body: rule) *)
+(*         (tau tau': type), *)
+(*         MaxType Gamma expr tau' -> *)
+(*         MaxType (putenv getenv Gamma var = Some tau') body tau -> *)
+(*         MaxType Gamma (Bind var expr body) tau *)
+(*   | MaxTypeVar: *)
+(*       forall (Gamma: varenv_t) *)
+(*         (var: var_t) *)
+(*         (tau: type), *)
+(*         getenv Gamma var = Some tau -> *)
+(*         MaxType Gamma (Var var) tau *)
+(*   | MaxTypeSkip: *)
+(*       forall (Gamma: varenv_t), *)
+(*         MaxType Gamma Skip (bits_t 0) *)
+(*   | MaxTypeConst: *)
+(*       forall (Gamma: varenv_t) *)
+(*         (cst: bits), *)
+(*         MaxType Gamma (Const cst) (bits_t (length cst)) *)
+(*   | MaxTypeIfF: *)
+(*       forall (Gamma: varenv_t) *)
+(*         (cond: rule) (tbranch: rule) (fbranch: rule) *)
+(*         (tauf taut: type), *)
+(*         HasType Gamma cond (bits_t 1) -> *)
+(*         MaxType Gamma tbranch taut -> *)
+(*         MaxType Gamma fbranch tauf -> *)
+(*         type_le tauf taut -> *)
+(*         MaxType Gamma (If cond tbranch fbranch) tauf *)
+(*   | MaxTypeIfT: *)
+(*       forall (Gamma: varenv_t) *)
+(*         (cond: rule) (tbranch: rule) (fbranch: rule) *)
+(*         (tauf taut: type), *)
+(*         HasType Gamma cond (bits_t 1) -> *)
+(*         MaxType Gamma tbranch taut -> *)
+(*         MaxType Gamma fbranch tauf -> *)
+(*         type_le taut tauf -> *)
+(*         MaxType Gamma (If cond tbranch fbranch) taut *)
+(*   | MaxTypeFail: *)
+(*       forall (Gamma: varenv_t), *)
+(*         MaxType Gamma Fail any_t *)
+(*   | MaxTypeRead: *)
+(*       forall (Gamma: varenv_t) *)
+(*         (port: Port) (idx: reg_t) *)
+(*         (size: nat) (n: nat), *)
+(*         R idx = size -> *)
+(*         MaxType Gamma (Read port idx) (bits_t size) *)
+(*   | MaxTypeWrite: *)
+(*       forall (Gamma: varenv_t) *)
+(*         (port: Port) (idx: reg_t) (value: rule) *)
+(*         (size: nat) (n: nat), *)
+(*         R idx = size -> *)
+(*         HasType Gamma value (bits_t size) -> *)
+(*         MaxType Gamma (Write port idx value) (bits_t 0) *)
+(*   | MaxTypeCall: *)
+(*       forall (Gamma: varenv_t) *)
+(*         (idx: fn_t) (a1 a2: rule) *)
+(*         (s1 s2: type) (retType: type), *)
+(*         Sigma idx = FunSig s1 s2 retType -> *)
+(*         HasType Gamma a1 (bits_t s1) -> *)
+(*         HasType Gamma a2 (bits_t s2) -> *)
+(*         MaxType Gamma (Call idx a1 a2) (bits_t retType). *)
+
+(*   Hint Constructors MaxType : types. *)
+
+(*   Theorem maxtypes_unicity : *)
+(*     forall Gamma s tau, *)
+(*       MaxType Gamma s tau -> *)
+(*       forall tau', *)
+(*         MaxType Gamma s tau' -> *)
+(*         tau = tau'. *)
+(*   Proof. *)
+(*     induction 1; intros * HasType'; *)
+(*       inversion HasType'; subst. *)
+(*     1-12: solve [firstorder (subst; firstorder (congruence || teauto))]. *)
+(*   Qed. *)
+
+(*   Hint Resolve maxtypes_unicity : types. *)
+
+(*   Lemma MaxType_HasType : forall Gamma s tau', MaxType Gamma s tau' -> forall tau, type_le tau tau' -> HasType Gamma s tau. *)
+(*     induction 1; teauto. *)
+(*   Qed. *)
+
+(*   Notation "Gamma [ k ↦ R ]" := *)
+(*     (putenv Gamma k R) (at level 7, left associativity, format "Gamma [ k  ↦  R ]"). *)
+(*   Notation "Gamma ⊢ s :: tau" := *)
+(*     (HasType Gamma s tau) (at level 8, no associativity). *)
+(*   Notation "Gamma ⊩ s :: tau" := *)
+(*     (MaxType Gamma s tau) (at level 8, no associativity). *)
+
+(*   Notation "tau ⩽ tau'" := *)
+(*     (type_le tau tau') (at level 10, no associativity). *)
+
+(*   Ltac t := *)
+(*     repeat match goal with *)
+(*            | [ H: fn ?Gamma ?k ?R, Hle: fenv_le ?Gamma _ |- _ ] => *)
+(*              pose_once Hle k R H *)
+(*            | [ H: exists _, _ |- _ ] => destruct H *)
+(*            | [ H: _ /\ _ |- _ ] => destruct H *)
+(*            end. *)
+
+(*   Lemma MaxType_increasing'' : forall s Gamma tau, *)
+(*       MaxType Gamma s tau -> *)
+(*       forall (Gamma': tenv var_t), *)
+(*         fenv_le Gamma Gamma' -> *)
+(*         exists tau', *)
+(*           MaxType Gamma' s tau' /\ *)
+(*           type_le tau tau'. *)
+(*   Proof. *)
+(*     induction 1; intros * le; t; teauto 6. *)
+
+(*     - specialize (IHMaxType1 _ le). *)
+(*       t. *)
+(*       assert (fenv_le Gamma[var ↦ tau'] Gamma'[var ↦ x]) as Hdiff. *)
+(*       { apply putenv_increasing; eassumption. } *)
+(*       specialize (IHMaxType2 _ Hdiff). *)
+(*       t. *)
+(*       teauto. *)
+
+(*     - specialize (IHMaxType1 _ le). *)
+(*       t. *)
+(*       specialize (IHMaxType2 _ le). *)
+(*       t. *)
+
+(*       destruct (type_le_upper_bounds_comparable *)
+(*                   tauf taut _ _ *)
+(*                   ltac:(eassumption) *)
+(*                   ltac:(eassumption) *)
+(*                   ltac:(eassumption)). *)
+(*       teauto. *)
+(*       teauto 6. *)
+
+(*     - specialize (IHMaxType1 _ le). *)
+(*       t. *)
+(*       specialize (IHMaxType2 _ le). *)
+(*       t. *)
+
+(*       destruct (type_le_upper_bounds_comparable *)
+(*                   taut tauf _ _ *)
+(*                   ltac:(eassumption) *)
+(*                   ltac:(eassumption) *)
+(*                   ltac:(eassumption)). *)
+(*       teauto. *)
+(*       teauto 6. *)
+(*     - teauto 8. *)
+(*   Qed. *)
+
+(*   Lemma HasType_MaxType : forall Gamma s tau, *)
+(*       HasType Gamma s tau -> *)
+(*       exists tau', MaxType Gamma s tau' /\ tau ⩽ tau'. *)
+(*   Proof. *)
+(*     induction 1; try solve [teauto || firstorder teauto]. *)
+(*     - t. *)
+
+(*       pose proof (MaxType_increasing'' *)
+(*                     _ _ _ H1 Gamma[var ↦ x0] *)
+(*                     ltac:(teauto)). *)
+(*       t. *)
+(*       teauto. *)
+(*     - t. *)
+
+(*       destruct (type_le_upper_bounds_comparable *)
+(*                   tau tau x x0 *)
+(*                   ltac:(teauto) *)
+(*                   ltac:(eassumption) *)
+(*                   ltac:(eassumption)). *)
+(*       teauto. *)
+(*       teauto. *)
+(*   Qed. *)
+
+(*   Hint Resolve MaxType_HasType : types. *)
+
+(*   Theorem types_unicity : *)
+(*     forall Gamma s tau, *)
+(*       HasType Gamma s tau -> *)
+(*       HasType Gamma s any_t \/ *)
+(*       forall tau', HasType Gamma s tau' -> tau = tau'. *)
+(*   Proof. *)
+(*     intros Gamma s tau H. *)
+(*     pose proof (HasType_MaxType _ _ _ H). *)
+(*     t. *)
+(*     destruct (type_eq_dec x any_t); subst. *)
+(*     - teauto. *)
+(*     - right. *)
+(*       intros tau' H'. *)
+(*       pose proof (HasType_MaxType _ _ _ H'). *)
+(*       t. *)
+(*       assert (x = x0) by teauto; subst. *)
+
+(*       transitivity x0. *)
+(*       teauto. *)
+(*       teauto. *)
+(*   Qed. *)
+
+(*   Notation scheduler := (scheduler var_t reg_t fn_t). *)
+
+(*   Inductive SchedulerHasTypes: forall (s: scheduler), Prop := *)
+(*   | SchedulerHasTypesDone : SchedulerHasTypes Done *)
+(*   | SchedulerHasTypesTry : *)
+(*       forall r tau s1 s2, *)
+(*         HasType fenv_nil r tau -> *)
+(*         SchedulerHasTypes s1 -> *)
+(*         SchedulerHasTypes s2 -> *)
+(*         SchedulerHasTypes (ry r s1 s2). *)
+(* End TC. *)
